Cleaner defnition of isim

src/Weakest.v
@@ -44,9 +44,7 @@ Section SIM.
   Variable tid: thread_id.
   Variable I: shared_rel.
 
-  Let rel := (forall R_src R_tgt (Q: R_src -> R_tgt -> shared_rel), bool -> bool -> itree srcE R_src -> itree tgtE R_tgt -> shared_rel).
-
-  Let coind :=  (bool * bool * rel * rel)%type.
+  Let rel := (forall R_src R_tgt (Q: R_src -> R_tgt -> shared_rel), itree srcE R_src -> itree tgtE R_tgt -> shared_rel).
 
   Let gf := (fun r => pind9 (__lsim (lift I) tid r) top9).
   Let gf_mon: monotone9 gf.
@@ -55,7 +53,7 @@ Section SIM.
   Qed.
   Hint Resolve gf_mon: paco.
 
-  Program Definition unlift (r: rel):
+  Variant unlift (r: rel):
     forall R_src R_tgt (RR: R_src -> R_tgt -> Σ ->
                             (TIdSet.t *
                                (@imap ident_src wf_src) *
@@ -68,45 +66,24 @@ Section SIM.
          (@imap (sum_tid ident_tgt) nat_wf) *
          state_src *
          state_tgt) -> Prop :=
-    (fun R_src R_tgt RR ps pt r_ctx itr_src itr_tgt '(ths, im_src, im_tgt, st_src, st_tgt) => exists r_own,
-         (<<WF: URA.wf (r_own ⋅ r_ctx)>>) /\
-           (<<SAT: @r _ _ (fun r_src r_tgt ths im_src im_tgt st_src st_tgt =>
-                             @iProp_intro _ (fun r_own => forall (r_ctx: Σ) (WF: URA.wf (r_own ⋅ r_ctx)),                                                                                     RR r_src r_tgt r_ctx (ths, im_src, im_tgt, st_src, st_tgt)) _) ps pt itr_src itr_tgt ths im_src im_tgt st_src st_tgt r_own>>)).
-  Next Obligation.
-  Proof.
-    i. ss. i. eapply H.
-    eapply URA.wf_extends; eauto. eapply URA.extends_add; eauto.
-  Qed.
-
-  Variant unlift2 (r: rel):
-    forall R_src R_tgt (RR: R_src -> R_tgt -> Σ ->
-                            (TIdSet.t *
-                               (@imap ident_src wf_src) *
-                               (@imap (sum_tid ident_tgt) nat_wf) *
-                               state_src *
-                               state_tgt) -> Prop),
-      bool -> bool -> Σ -> itree srcE R_src -> itree tgtE R_tgt ->
-      (TIdSet.t *
-         (@imap ident_src wf_src) *
-         (@imap (sum_tid ident_tgt) nat_wf) *
-         state_src *
-         state_tgt) -> Prop :=
-    | unlift2_intro
+    | unlift_intro
         R_src R_tgt Q ps pt itr_src itr_tgt ths im_src im_tgt st_src st_tgt r_ctx r_own
-        (REL: r R_src R_tgt Q ps pt itr_src itr_tgt ths im_src im_tgt st_src st_tgt r_own)
+        (REL: r R_src R_tgt Q itr_src itr_tgt ths im_src im_tgt st_src st_tgt r_own)
         (WF: URA.wf (r_own ⋅ r_ctx))
+        (PS: ps = false)
+        (PT: pt = false)
       :
-      unlift2 r (liftRR Q) ps pt r_ctx itr_src itr_tgt (ths, im_src, im_tgt, st_src, st_tgt)
+      unlift r (liftRR Q) ps pt r_ctx itr_src itr_tgt (ths, im_src, im_tgt, st_src, st_tgt)
   .
 
   Program Definition isim: rel -> rel -> rel :=
     fun
       r g
-      R_src R_tgt Q ps pt itr_src itr_tgt ths im_src im_tgt st_src st_tgt =>
+      R_src R_tgt Q itr_src itr_tgt ths im_src im_tgt st_src st_tgt =>
       iProp_intro
         (fun r_own =>
            forall r_ctx (WF: URA.wf (r_own ⋅ r_ctx)),
-             gpaco9 gf (cpn9 gf) (@unlift2 r) (@unlift2 g) _ _ (liftRR Q) ps pt r_ctx itr_src itr_tgt (ths, im_src, im_tgt, st_src, st_tgt)) _.
+             gpaco9 gf (cpn9 gf) (@unlift r) (@unlift g) _ _ (liftRR Q) false false r_ctx itr_src itr_tgt (ths, im_src, im_tgt, st_src, st_tgt)) _.
   Next Obligation.
   Proof.
     ii. ss. eapply H.
@@ -116,7 +93,7 @@ Section SIM.
   Tactic Notation "muclo" uconstr(H) :=
     eapply gpaco9_uclo; [auto with paco|apply H|].
 
-  Lemma isim_mono ps pt r g R_src R_tgt
+  Lemma isim_mono r g R_src R_tgt
         (Q0 Q1: R_src -> R_tgt -> shared_rel)
         (MONO: forall r_src r_tgt ths im_src im_tgt st_src st_tgt,
             bi_entails
@@ -125,8 +102,8 @@ Section SIM.
         itr_src itr_tgt ths im_src im_tgt st_src st_tgt
     :
     bi_entails
-      (isim r g Q0 ps pt itr_src itr_tgt ths im_src im_tgt st_src st_tgt)
-      (isim r g Q1 ps pt itr_src itr_tgt ths im_src im_tgt st_src st_tgt)
+      (isim r g Q0 itr_src itr_tgt ths im_src im_tgt st_src st_tgt)
+      (isim r g Q1 itr_src itr_tgt ths im_src im_tgt st_src st_tgt)
   .
   Proof.
     rr. autorewrite with iprop. i.
@@ -142,13 +119,13 @@ Section SIM.
     hexploit (H0 r_ctx0); eauto.
   Qed.
 
-  Lemma isim_upd ps pt r g R_src R_tgt
+  Lemma isim_upd r g R_src R_tgt
         (Q: R_src -> R_tgt -> shared_rel)
         itr_src itr_tgt ths im_src im_tgt st_src st_tgt
     :
     bi_entails
-      (#=> (isim r g Q ps pt itr_src itr_tgt ths im_src im_tgt st_src st_tgt))
-      (isim r g Q ps pt itr_src itr_tgt ths im_src im_tgt st_src st_tgt)
+      (#=> (isim r g Q itr_src itr_tgt ths im_src im_tgt st_src st_tgt))
+      (isim r g Q itr_src itr_tgt ths im_src im_tgt st_src st_tgt)
   .
   Proof.
     rr. autorewrite with iprop. i.
@@ -156,30 +133,14 @@ Section SIM.
     ii. hexploit H; eauto. i. des. eauto.
   Qed.
 
-  Lemma isim_reset ps0 pt0 ps1 pt1 r g R_src R_tgt
-        (Q: R_src -> R_tgt -> shared_rel)
-        itr_src itr_tgt ths im_src im_tgt st_src st_tgt
-        (PS: ps0 = true -> ps1 = true)
-        (PT: pt0 = true -> pt1 = true)
-    :
-    bi_entails
-      (isim r g Q ps0 pt0 itr_src itr_tgt ths im_src im_tgt st_src st_tgt)
-      (isim r g Q ps1 pt1 itr_src itr_tgt ths im_src im_tgt st_src st_tgt)
-  .
-  Proof.
-    rr. autorewrite with iprop. i.
-    ii. muclo lsim_resetC_spec.
-    econs; eauto.
-  Qed.
-
-  Lemma isim_wand ps pt r g R_src R_tgt
+  Lemma isim_wand r g R_src R_tgt
         (Q0 Q1: R_src -> R_tgt -> shared_rel)
         itr_src itr_tgt ths im_src im_tgt st_src st_tgt
     :
     bi_entails
       ((∀ r_src r_tgt ths im_src im_tgt st_src st_tgt,
-           ((Q0 r_src r_tgt ths im_src im_tgt st_src st_tgt) -∗ (Q1 r_src r_tgt ths im_src im_tgt st_src st_tgt))) ** (isim r g Q0 ps pt itr_src itr_tgt ths im_src im_tgt st_src st_tgt))
-      (isim r g Q1 ps pt itr_src itr_tgt ths im_src im_tgt st_src st_tgt)
+           ((Q0 r_src r_tgt ths im_src im_tgt st_src st_tgt) -∗ (Q1 r_src r_tgt ths im_src im_tgt st_src st_tgt))) ** (isim r g Q0 itr_src itr_tgt ths im_src im_tgt st_src st_tgt))
+      (isim r g Q1 itr_src itr_tgt ths im_src im_tgt st_src st_tgt)
   .
   Proof.
     rr. autorewrite with iprop. i.
@@ -207,7 +168,7 @@ Section SIM.
     }
   Qed.
 
-  Lemma isim_bind ps pt r g R_src R_tgt S_src S_tgt
+  Lemma isim_bind r g R_src R_tgt S_src S_tgt
         (Q: R_src -> R_tgt -> shared_rel)
         (itr_src: itree srcE S_src) (itr_tgt: itree tgtE S_tgt)
         ktr_src ktr_tgt
@@ -215,8 +176,8 @@ Section SIM.
     :
     bi_entails
       (isim r g (fun s_src s_tgt ths im_src im_tgt st_src st_tgt =>
-                   isim r g Q false false (ktr_src s_src) (ktr_tgt s_tgt) ths im_src im_tgt st_src st_tgt) ps pt itr_src itr_tgt ths im_src im_tgt st_src st_tgt)
-      (isim r g Q ps pt (itr_src >>= ktr_src) (itr_tgt >>= ktr_tgt) ths im_src im_tgt st_src st_tgt)
+                   isim r g Q (ktr_src s_src) (ktr_tgt s_tgt) ths im_src im_tgt st_src st_tgt) itr_src itr_tgt ths im_src im_tgt st_src st_tgt)
+      (isim r g Q (itr_src >>= ktr_src) (itr_tgt >>= ktr_tgt) ths im_src im_tgt st_src st_tgt)
   .
   Proof.
     rr. autorewrite with iprop. i.
@@ -232,27 +193,13 @@ Section SIM.
     unfold liftRR. i. des_ifs.
   Qed.
 
-  Lemma isim_progress r g R_src R_tgt
-        (Q: R_src -> R_tgt -> shared_rel)
-        itr_src itr_tgt ths im_src im_tgt st_src st_tgt
-    :
-    bi_entails
-      (isim g g Q false false itr_src itr_tgt ths im_src im_tgt st_src st_tgt)
-      (isim r g Q true true itr_src itr_tgt ths im_src im_tgt st_src st_tgt)
-  .
-  Proof.
-    rr. autorewrite with iprop.
-    ii. gstep. rr. eapply pind9_fold.
-    eapply lsim_progress; eauto.
-  Qed.
-
-  Lemma isim_ret ps pt r g R_src R_tgt
+  Lemma isim_ret r g R_src R_tgt
         (Q: R_src -> R_tgt -> shared_rel)
         r_src r_tgt ths im_src im_tgt st_src st_tgt
     :
     bi_entails
       (Q r_src r_tgt ths im_src im_tgt st_src st_tgt)
-      (isim r g Q ps pt (Ret r_src) (Ret r_tgt) ths im_src im_tgt st_src st_tgt)
+      (isim r g Q (Ret r_src) (Ret r_tgt) ths im_src im_tgt st_src st_tgt)
   .
   Proof.
     rr. autorewrite with iprop. i.
@@ -260,157 +207,157 @@ Section SIM.
     eapply lsim_ret. unfold liftRR. esplits; eauto.
   Qed.
 
-  Lemma isim_tauL ps pt r g R_src R_tgt
+  Lemma isim_tauL r g R_src R_tgt
         (Q: R_src -> R_tgt -> shared_rel)
         itr_src itr_tgt ths im_src im_tgt st_src st_tgt
     :
     bi_entails
-      (isim r g Q true pt itr_src itr_tgt ths im_src im_tgt st_src st_tgt)
-      (isim r g Q ps pt (Tau itr_src) itr_tgt ths im_src im_tgt st_src st_tgt)
+      (isim r g Q itr_src itr_tgt ths im_src im_tgt st_src st_tgt)
+      (isim r g Q (Tau itr_src) itr_tgt ths im_src im_tgt st_src st_tgt)
   .
   Proof.
     rr. autorewrite with iprop. i.
     ii. muclo lsim_indC_spec.
-    eapply lsim_tauL. eapply H; eauto.
+    eapply lsim_tauL. muclo lsim_resetC_spec. econs; eauto.
   Qed.
 
-  Lemma isim_tauR ps pt r g R_src R_tgt
+  Lemma isim_tauR r g R_src R_tgt
         (Q: R_src -> R_tgt -> shared_rel)
         itr_src itr_tgt ths im_src im_tgt st_src st_tgt
     :
     bi_entails
-      (isim r g Q ps true itr_src itr_tgt ths im_src im_tgt st_src st_tgt)
-      (isim r g Q ps pt itr_src (Tau itr_tgt) ths im_src im_tgt st_src st_tgt)
+      (isim r g Q itr_src itr_tgt ths im_src im_tgt st_src st_tgt)
+      (isim r g Q itr_src (Tau itr_tgt) ths im_src im_tgt st_src st_tgt)
   .
   Proof.
     rr. autorewrite with iprop. i.
     ii. muclo lsim_indC_spec.
-    eapply lsim_tauR. eapply H; eauto.
+    eapply lsim_tauR. muclo lsim_resetC_spec. econs; eauto.
   Qed.
 
-  Lemma isim_chooseL X ps pt r g R_src R_tgt
+  Lemma isim_chooseL X r g R_src R_tgt
         (Q: R_src -> R_tgt -> shared_rel)
         ktr_src itr_tgt ths im_src im_tgt st_src st_tgt
     :
     bi_entails
-      (∃ x, isim r g Q true pt (ktr_src x) itr_tgt ths im_src im_tgt st_src st_tgt)
-      (isim r g Q ps pt (trigger (Choose X) >>= ktr_src) itr_tgt ths im_src im_tgt st_src st_tgt)
+      (∃ x, isim r g Q (ktr_src x) itr_tgt ths im_src im_tgt st_src st_tgt)
+      (isim r g Q (trigger (Choose X) >>= ktr_src) itr_tgt ths im_src im_tgt st_src st_tgt)
   .
   Proof.
     rr. autorewrite with iprop. i.
     ii. muclo lsim_indC_spec.
     eapply lsim_chooseL.
     rr in H. autorewrite with iprop in H. des.
-    esplits; eauto.
+    esplits; eauto. muclo lsim_resetC_spec. econs; eauto.
   Qed.
 
-  Lemma isim_chooseR X ps pt r g R_src R_tgt
+  Lemma isim_chooseR X r g R_src R_tgt
         (Q: R_src -> R_tgt -> shared_rel)
         itr_src ktr_tgt ths im_src im_tgt st_src st_tgt
     :
     bi_entails
-      (∀ x, isim r g Q ps true itr_src (ktr_tgt x) ths im_src im_tgt st_src st_tgt)
-      (isim r g Q ps pt itr_src (trigger (Choose X) >>= ktr_tgt) ths im_src im_tgt st_src st_tgt)
+      (∀ x, isim r g Q itr_src (ktr_tgt x) ths im_src im_tgt st_src st_tgt)
+      (isim r g Q itr_src (trigger (Choose X) >>= ktr_tgt) ths im_src im_tgt st_src st_tgt)
   .
   Proof.
     rr. autorewrite with iprop. i.
     ii. muclo lsim_indC_spec.
     eapply lsim_chooseR.
     rr in H. autorewrite with iprop in H.
-    i. eapply H; eauto.
+    i. muclo lsim_resetC_spec. econs; [eapply H|..]; eauto.
   Qed.
 
-  Lemma isim_putL st ps pt r g R_src R_tgt
+  Lemma isim_putL st r g R_src R_tgt
         (Q: R_src -> R_tgt -> shared_rel)
         ktr_src itr_tgt ths im_src im_tgt st_src st_tgt
     :
     bi_entails
-      (isim r g Q true pt (ktr_src tt) itr_tgt ths im_src im_tgt st st_tgt)
-      (isim r g Q ps pt (trigger (Put st) >>= ktr_src) itr_tgt ths im_src im_tgt st_src st_tgt)
+      (isim r g Q (ktr_src tt) itr_tgt ths im_src im_tgt st st_tgt)
+      (isim r g Q (trigger (Put st) >>= ktr_src) itr_tgt ths im_src im_tgt st_src st_tgt)
   .
   Proof.
     rr. autorewrite with iprop. i.
     ii. muclo lsim_indC_spec.
-    eapply lsim_putL. eapply H; eauto.
+    eapply lsim_putL. muclo lsim_resetC_spec. econs; [eapply H|..]; eauto.
   Qed.
 
-  Lemma isim_putR st ps pt r g R_src R_tgt
+  Lemma isim_putR st r g R_src R_tgt
         (Q: R_src -> R_tgt -> shared_rel)
         itr_src ktr_tgt ths im_src im_tgt st_src st_tgt
     :
     bi_entails
-      (isim r g Q ps true itr_src (ktr_tgt tt) ths im_src im_tgt st_src st)
-      (isim r g Q ps pt itr_src (trigger (Put st) >>= ktr_tgt) ths im_src im_tgt st_src st_tgt)
+      (isim r g Q itr_src (ktr_tgt tt) ths im_src im_tgt st_src st)
+      (isim r g Q itr_src (trigger (Put st) >>= ktr_tgt) ths im_src im_tgt st_src st_tgt)
   .
   Proof.
     rr. autorewrite with iprop. i.
     ii. muclo lsim_indC_spec.
-    eapply lsim_putR. eapply H; eauto.
+    eapply lsim_putR. muclo lsim_resetC_spec. econs; [eapply H|..]; eauto.
   Qed.
 
-  Lemma isim_getL ps pt r g R_src R_tgt
+  Lemma isim_getL r g R_src R_tgt
         (Q: R_src -> R_tgt -> shared_rel)
         ktr_src itr_tgt ths im_src im_tgt st_src st_tgt
     :
     bi_entails
-      (isim r g Q true pt (ktr_src st_src) itr_tgt ths im_src im_tgt st_src st_tgt)
-      (isim r g Q ps pt (trigger (@Get _) >>= ktr_src) itr_tgt ths im_src im_tgt st_src st_tgt)
+      (isim r g Q (ktr_src st_src) itr_tgt ths im_src im_tgt st_src st_tgt)
+      (isim r g Q (trigger (@Get _) >>= ktr_src) itr_tgt ths im_src im_tgt st_src st_tgt)
   .
   Proof.
     rr. autorewrite with iprop. i.
     ii. muclo lsim_indC_spec.
-    eapply lsim_getL. eapply H; eauto.
+    eapply lsim_getL. muclo lsim_resetC_spec. econs; [eapply H|..]; eauto.
   Qed.
 
-  Lemma isim_getR ps pt r g R_src R_tgt
+  Lemma isim_getR r g R_src R_tgt
         (Q: R_src -> R_tgt -> shared_rel)
         itr_src ktr_tgt ths im_src im_tgt st_src st_tgt
     :
     bi_entails
-      (isim r g Q ps true itr_src (ktr_tgt st_tgt) ths im_src im_tgt st_src st_tgt)
-      (isim r g Q ps pt itr_src (trigger (@Get _) >>= ktr_tgt) ths im_src im_tgt st_src st_tgt)
+      (isim r g Q itr_src (ktr_tgt st_tgt) ths im_src im_tgt st_src st_tgt)
+      (isim r g Q itr_src (trigger (@Get _) >>= ktr_tgt) ths im_src im_tgt st_src st_tgt)
   .
   Proof.
     rr. autorewrite with iprop. i.
     ii. muclo lsim_indC_spec.
-    eapply lsim_getR. eapply H; eauto.
+    eapply lsim_getR. muclo lsim_resetC_spec. econs; [eapply H|..]; eauto.
   Qed.
 
-  Lemma isim_tidL ps pt r g R_src R_tgt
+  Lemma isim_tidL r g R_src R_tgt
         (Q: R_src -> R_tgt -> shared_rel)
         ktr_src itr_tgt ths im_src im_tgt st_src st_tgt
     :
     bi_entails
-      (isim r g Q true pt (ktr_src tid) itr_tgt ths im_src im_tgt st_src st_tgt)
-      (isim r g Q ps pt (trigger GetTid >>= ktr_src) itr_tgt ths im_src im_tgt st_src st_tgt)
+      (isim r g Q (ktr_src tid) itr_tgt ths im_src im_tgt st_src st_tgt)
+      (isim r g Q (trigger GetTid >>= ktr_src) itr_tgt ths im_src im_tgt st_src st_tgt)
   .
   Proof.
     rr. autorewrite with iprop. i.
     ii. muclo lsim_indC_spec.
-    eapply lsim_tidL. eapply H; eauto.
+    eapply lsim_tidL. muclo lsim_resetC_spec. econs; [eapply H|..]; eauto.
   Qed.
 
-  Lemma isim_tidR ps pt r g R_src R_tgt
+  Lemma isim_tidR r g R_src R_tgt
         (Q: R_src -> R_tgt -> shared_rel)
         itr_src ktr_tgt ths im_src im_tgt st_src st_tgt
     :
     bi_entails
-      (isim r g Q ps true itr_src (ktr_tgt tid) ths im_src im_tgt st_src st_tgt)
-      (isim r g Q ps pt itr_src (trigger GetTid >>= ktr_tgt) ths im_src im_tgt st_src st_tgt)
+      (isim r g Q itr_src (ktr_tgt tid) ths im_src im_tgt st_src st_tgt)
+      (isim r g Q itr_src (trigger GetTid >>= ktr_tgt) ths im_src im_tgt st_src st_tgt)
   .
   Proof.
     rr. autorewrite with iprop. i.
     ii. muclo lsim_indC_spec.
-    eapply lsim_tidR. eapply H; eauto.
+    eapply lsim_tidR. muclo lsim_resetC_spec. econs; [eapply H|..]; eauto.
   Qed.
 
-  Lemma isim_fairL f ps pt r g R_src R_tgt
+  Lemma isim_fairL f r g R_src R_tgt
         (Q: R_src -> R_tgt -> shared_rel)
         ktr_src itr_tgt ths im_src0 im_tgt st_src st_tgt
     :
     bi_entails
-      (∃ im_src1, ⌜fair_update im_src0 im_src1 f⌝ ∧ isim r g Q true pt (ktr_src tt) itr_tgt ths im_src1 im_tgt st_src st_tgt)
-      (isim r g Q ps pt (trigger (Fair f) >>= ktr_src) itr_tgt ths im_src0 im_tgt st_src st_tgt)
+      (∃ im_src1, ⌜fair_update im_src0 im_src1 f⌝ ∧ isim r g Q (ktr_src tt) itr_tgt ths im_src1 im_tgt st_src st_tgt)
+      (isim r g Q (trigger (Fair f) >>= ktr_src) itr_tgt ths im_src0 im_tgt st_src st_tgt)
   .
   Proof.
     rr. autorewrite with iprop. i.
@@ -419,16 +366,16 @@ Section SIM.
     rr in H. autorewrite with iprop in H. des.
     rr in H. autorewrite with iprop in H. des.
     rr in H. autorewrite with iprop in H.
-    esplits; eauto.
+    esplits; eauto. muclo lsim_resetC_spec. econs; [eapply H0|..]; eauto.
   Qed.
 
-  Lemma isim_fairR f ps pt r g R_src R_tgt
+  Lemma isim_fairR f r g R_src R_tgt
         (Q: R_src -> R_tgt -> shared_rel)
         itr_src ktr_tgt ths im_src im_tgt0 st_src st_tgt
     :
     bi_entails
-      (∀ im_tgt1, ⌜fair_update im_tgt0 im_tgt1 (sum_fmap_r f)⌝ -* isim r g Q ps true itr_src (ktr_tgt tt) ths im_src im_tgt1 st_src st_tgt)
-      (isim r g Q ps pt itr_src (trigger (Fair f) >>= ktr_tgt) ths im_src im_tgt0 st_src st_tgt)
+      (∀ im_tgt1, ⌜fair_update im_tgt0 im_tgt1 (sum_fmap_r f)⌝ -* isim r g Q itr_src (ktr_tgt tt) ths im_src im_tgt1 st_src st_tgt)
+      (isim r g Q itr_src (trigger (Fair f) >>= ktr_tgt) ths im_src im_tgt0 st_src st_tgt)
   .
   Proof.
     rr. autorewrite with iprop. i.
@@ -440,16 +387,16 @@ Section SIM.
     hexploit (H0 URA.unit); eauto.
     { rewrite URA.unit_id. eapply URA.wf_mon; eauto. }
     { rr. autorewrite with iprop. eauto. }
-    i. eapply H1; eauto. rewrite URA.unit_id. auto.
+    i. muclo lsim_resetC_spec. econs; [eapply H1|..]; eauto. r_wf WF0.
   Qed.
 
-  Lemma isim_UB ps pt r g R_src R_tgt
+  Lemma isim_UB r g R_src R_tgt
         (Q: R_src -> R_tgt -> shared_rel)
         ktr_src itr_tgt ths im_src im_tgt st_src st_tgt
     :
     bi_entails
       (True)
-      (isim r g Q ps pt (trigger Undefined >>= ktr_src) itr_tgt ths im_src im_tgt st_src st_tgt)
+      (isim r g Q (trigger Undefined >>= ktr_src) itr_tgt ths im_src im_tgt st_src st_tgt)
   .
   Proof.
     rr. autorewrite with iprop. i.
@@ -457,43 +404,43 @@ Section SIM.
     eapply lsim_UB.
   Qed.
 
-  Lemma isim_observe fn args ps pt r g R_src R_tgt
+  Lemma isim_observe fn args r g R_src R_tgt
         (Q: R_src -> R_tgt -> shared_rel)
         ktr_src ktr_tgt ths im_src im_tgt st_src st_tgt
     :
     bi_entails
-      (∀ ret, isim g g Q true true (ktr_src ret) (ktr_tgt ret) ths im_src im_tgt st_src st_tgt)
-      (isim r g Q ps pt (trigger (Observe fn args) >>= ktr_src) (trigger (Observe fn args) >>= ktr_tgt) ths im_src im_tgt st_src st_tgt)
+      (∀ ret, isim g g Q (ktr_src ret) (ktr_tgt ret) ths im_src im_tgt st_src st_tgt)
+      (isim r g Q (trigger (Observe fn args) >>= ktr_src) (trigger (Observe fn args) >>= ktr_tgt) ths im_src im_tgt st_src st_tgt)
   .
   Proof.
     rr. autorewrite with iprop. i.
     ii. gstep. rr. eapply pind9_fold.
     eapply lsim_observe; eauto.
     i. rr in H. autorewrite with iprop in H.
-    eapply H; eauto.
+    muclo lsim_resetC_spec. econs; [eapply H|..]; eauto.
   Qed.
 
-  Lemma isim_yieldL ps pt r g R_src R_tgt
+  Lemma isim_yieldL r g R_src R_tgt
         (Q: R_src -> R_tgt -> shared_rel)
         ktr_src ktr_tgt ths im_src im_tgt st_src st_tgt
     :
     bi_entails
-      (isim r g Q true pt (ktr_src tt) (trigger (Yield) >>= ktr_tgt) ths im_src im_tgt st_src st_tgt)
-      (isim r g Q ps pt (trigger (Yield) >>= ktr_src) (trigger (Yield) >>= ktr_tgt) ths im_src im_tgt st_src st_tgt)
+      (isim r g Q (ktr_src tt) (trigger (Yield) >>= ktr_tgt) ths im_src im_tgt st_src st_tgt)
+      (isim r g Q (trigger (Yield) >>= ktr_src) (trigger (Yield) >>= ktr_tgt) ths im_src im_tgt st_src st_tgt)
   .
   Proof.
     rr. autorewrite with iprop. i.
     ii. muclo lsim_indC_spec.
-    eapply lsim_yieldL. eapply H; eauto.
+    eapply lsim_yieldL. muclo lsim_resetC_spec. econs; [eapply H|..]; eauto.
   Qed.
 
-  Lemma isim_yieldR ps pt r g R_src R_tgt
+  Lemma isim_yieldR r g R_src R_tgt
         (Q: R_src -> R_tgt -> shared_rel)
         ktr_src ktr_tgt ths0 im_src0 im_tgt0 st_src0 st_tgt0
     :
     bi_entails
-      (I ths0 im_src0 im_tgt0 st_src0 st_tgt0 ** (∀ ths1 im_src1 im_tgt1 st_src1 st_tgt1 im_tgt2, I ths1 im_src1 im_tgt1 st_src1 st_tgt1 -* ⌜fair_update im_tgt1 im_tgt2 (sum_fmap_l (tids_fmap tid ths1))⌝ -* isim r g Q ps true (trigger (Yield) >>= ktr_src) (ktr_tgt tt) ths1 im_src1 im_tgt2 st_src1 st_tgt1))
-      (isim r g Q ps pt (trigger (Yield) >>= ktr_src) (trigger (Yield) >>= ktr_tgt) ths0 im_src0 im_tgt0 st_src0 st_tgt0)
+      (I ths0 im_src0 im_tgt0 st_src0 st_tgt0 ** (∀ ths1 im_src1 im_tgt1 st_src1 st_tgt1 im_tgt2, I ths1 im_src1 im_tgt1 st_src1 st_tgt1 -* ⌜fair_update im_tgt1 im_tgt2 (sum_fmap_l (tids_fmap tid ths1))⌝ -* isim r g Q (trigger (Yield) >>= ktr_src) (ktr_tgt tt) ths1 im_src1 im_tgt2 st_src1 st_tgt1))
+      (isim r g Q (trigger (Yield) >>= ktr_src) (trigger (Yield) >>= ktr_tgt) ths0 im_src0 im_tgt0 st_src0 st_tgt0)
   .
   Proof.
     rr. autorewrite with iprop. i.
@@ -512,16 +459,16 @@ Section SIM.
     i. rr in H. autorewrite with iprop in H. hexploit (H URA.unit); eauto.
     { eapply URA.wf_mon. instantiate (1:=r_ctx1). r_wf VALID. }
     { rr. autorewrite with iprop. eauto. }
-    i. eapply H2. r_wf VALID.
+    i. muclo lsim_resetC_spec. econs; [eapply H2|..]; eauto. r_wf VALID.
   Qed.
 
-  Lemma isim_sync ps pt r g R_src R_tgt
+  Lemma isim_sync r g R_src R_tgt
         (Q: R_src -> R_tgt -> shared_rel)
         ktr_src ktr_tgt ths0 im_src0 im_tgt0 st_src0 st_tgt0
     :
     bi_entails
-      (I ths0 im_src0 im_tgt0 st_src0 st_tgt0 ** (∀ ths1 im_src1 im_tgt1 st_src1 st_tgt1 im_tgt2, I ths1 im_src1 im_tgt1 st_src1 st_tgt1 -* ⌜fair_update im_tgt1 im_tgt2 (sum_fmap_l (tids_fmap tid ths1))⌝ -* isim g g Q true true (ktr_src tt) (ktr_tgt tt) ths1 im_src1 im_tgt2 st_src1 st_tgt1))
-      (isim r g Q ps pt (trigger (Yield) >>= ktr_src) (trigger (Yield) >>= ktr_tgt) ths0 im_src0 im_tgt0 st_src0 st_tgt0)
+      (I ths0 im_src0 im_tgt0 st_src0 st_tgt0 ** (∀ ths1 im_src1 im_tgt1 st_src1 st_tgt1 im_tgt2, I ths1 im_src1 im_tgt1 st_src1 st_tgt1 -* ⌜fair_update im_tgt1 im_tgt2 (sum_fmap_l (tids_fmap tid ths1))⌝ -* isim g g Q (ktr_src tt) (ktr_tgt tt) ths1 im_src1 im_tgt2 st_src1 st_tgt1))
+      (isim r g Q (trigger (Yield) >>= ktr_src) (trigger (Yield) >>= ktr_tgt) ths0 im_src0 im_tgt0 st_src0 st_tgt0)
   .
   Proof.
     rr. autorewrite with iprop. i.
@@ -539,16 +486,16 @@ Section SIM.
     i. rr in H. autorewrite with iprop in H. hexploit (H URA.unit); eauto.
     { eapply URA.wf_mon. instantiate (1:=r_ctx1). r_wf VALID. }
     { rr. autorewrite with iprop. eauto. }
-    i. eapply H2. r_wf VALID.
+    i. muclo lsim_resetC_spec. econs; [eapply H2|..]; eauto. r_wf VALID.
   Qed.
 
-  Lemma isim_base ps pt r g R_src R_tgt
+  Lemma isim_base r g R_src R_tgt
         (Q: R_src -> R_tgt -> shared_rel)
         itr_src itr_tgt ths im_src im_tgt st_src st_tgt
     :
     bi_entails
-      (@r _ _ Q ps pt itr_src itr_tgt ths im_src im_tgt st_src st_tgt)
-      (isim r g Q ps pt itr_src itr_tgt ths im_src im_tgt st_src st_tgt)
+      (@r _ _ Q itr_src itr_tgt ths im_src im_tgt st_src st_tgt)
+      (isim r g Q itr_src itr_tgt ths im_src im_tgt st_src st_tgt)
   .
   Proof.
     rr. autorewrite with iprop.
@@ -557,12 +504,12 @@ Section SIM.
 
   Lemma unlift_mon (r0 r1: rel)
         (MON: forall R_src R_tgt (Q: R_src -> R_tgt -> shared_rel)
-                     ps pt itr_src itr_tgt ths im_src im_tgt st_src st_tgt,
+                     itr_src itr_tgt ths im_src im_tgt st_src st_tgt,
             bi_entails
-              (@r0 _ _ Q ps pt itr_src itr_tgt ths im_src im_tgt st_src st_tgt)
-              (#=> (@r1 _ _ Q ps pt itr_src itr_tgt ths im_src im_tgt st_src st_tgt)))
+              (@r0 _ _ Q itr_src itr_tgt ths im_src im_tgt st_src st_tgt)
+              (#=> (@r1 _ _ Q itr_src itr_tgt ths im_src im_tgt st_src st_tgt)))
     :
-    unlift2 r0 <9= unlift2 r1.
+    unlift r0 <9= unlift r1.
   Proof.
     i. dependent destruction PR.
     hexploit MON; eauto. i.
@@ -573,23 +520,23 @@ Section SIM.
     hexploit H0; eauto. i. des. econs; eauto.
   Qed.
 
-  Lemma isim_mono_knowledge (r0 g0 r1 g1: rel) ps pt R_src R_tgt
+  Lemma isim_mono_knowledge (r0 g0 r1 g1: rel) R_src R_tgt
         (Q: R_src -> R_tgt -> shared_rel)
         itr_src itr_tgt ths im_src im_tgt st_src st_tgt
         (MON0: forall R_src R_tgt (Q: R_src -> R_tgt -> shared_rel)
-                      ps pt itr_src itr_tgt ths im_src im_tgt st_src st_tgt,
+                      itr_src itr_tgt ths im_src im_tgt st_src st_tgt,
             bi_entails
-              (@r0 _ _ Q ps pt itr_src itr_tgt ths im_src im_tgt st_src st_tgt)
-              (#=> (@r1 _ _ Q ps pt itr_src itr_tgt ths im_src im_tgt st_src st_tgt)))
+              (@r0 _ _ Q itr_src itr_tgt ths im_src im_tgt st_src st_tgt)
+              (#=> (@r1 _ _ Q itr_src itr_tgt ths im_src im_tgt st_src st_tgt)))
         (MON1: forall R_src R_tgt (Q: R_src -> R_tgt -> shared_rel)
-                      ps pt itr_src itr_tgt ths im_src im_tgt st_src st_tgt,
+                      itr_src itr_tgt ths im_src im_tgt st_src st_tgt,
             bi_entails
-              (@g0 _ _ Q ps pt itr_src itr_tgt ths im_src im_tgt st_src st_tgt)
-              (#=> (@g1 _ _ Q ps pt itr_src itr_tgt ths im_src im_tgt st_src st_tgt)))
+              (@g0 _ _ Q itr_src itr_tgt ths im_src im_tgt st_src st_tgt)
+              (#=> (@g1 _ _ Q itr_src itr_tgt ths im_src im_tgt st_src st_tgt)))
     :
     bi_entails
-      (isim r0 g0 Q ps pt itr_src itr_tgt ths im_src im_tgt st_src st_tgt)
-      (isim r1 g1 Q ps pt itr_src itr_tgt ths im_src im_tgt st_src st_tgt)
+      (isim r0 g0 Q itr_src itr_tgt ths im_src im_tgt st_src st_tgt)
+      (isim r1 g1 Q itr_src itr_tgt ths im_src im_tgt st_src st_tgt)
   .
   Proof.
     rr. autorewrite with iprop. i.
@@ -599,48 +546,7 @@ Section SIM.
     { eapply unlift_mon; eauto. }
   Qed.
 
-  Ltac espc H :=
-    let T := fresh "T" in
-    evar (T: Type);
-    let x := fresh "x" in
-    evar (x: T);
-    specialize (H x); subst T; subst x.
-
-  Tactic Notation "rspc" constr(H) := rr in H; autorewrite with iprop in H; espc H.
-  Ltac rspc := rr; autorewrite with iprop.
-
-  Goal forall (A B C: iProp),
-      bi_entails
-        (□ A)
-        A.
-  Proof.
-    i. iIntros "#H". iApply "H".
-  Qed.
-
-  Goal forall (A B C: iProp),
-      bi_entails
-        (□ (A -* B))
-        (□ (A → B))
-  .
-  Proof.
-    i. iIntros "#H". iModIntro.
-    iIntros "X". iApply "H". iApply "X".
-  Qed.
-
-  Goal forall (A B C: iProp),
-      bi_entails
-        (A → B)
-        (A -* B).
-  Proof.
-    i. iIntros "X Y".
-    iAssert (A ∧ (A → B))%I with "[X Y]" as "XX".
-    { iSplit; auto. }
-    iApply bi.impl_elim_r. eauto.
-  Qed.
-
   Lemma isim_coind A
-        (ps: forall (a: A), bool)
-        (pt: forall (a: A), bool)
         (R_src: forall (a: A), Prop)
         (R_tgt: forall (a: A), Prop)
         (Q: forall (a: A), R_src a -> R_tgt a -> shared_rel)
@@ -654,19 +560,19 @@ Section SIM.
         (P: forall (a: A), iProp)
         (r g0: rel)
         (COIND: forall (g1: rel) a, bi_entails (□((∀ R_src R_tgt (Q: R_src -> R_tgt -> shared_rel)
-                                                     ps pt itr_src itr_tgt ths im_src im_tgt st_src st_tgt,
-                                                      @g0 R_src R_tgt Q ps pt itr_src itr_tgt ths im_src im_tgt st_src st_tgt -* @g1 R_src R_tgt Q ps pt itr_src itr_tgt ths im_src im_tgt st_src st_tgt)
+                                                     itr_src itr_tgt ths im_src im_tgt st_src st_tgt,
+                                                      @g0 R_src R_tgt Q itr_src itr_tgt ths im_src im_tgt st_src st_tgt -* @g1 R_src R_tgt Q itr_src itr_tgt ths im_src im_tgt st_src st_tgt)
                                                     **
-                                                    (∀ a, P a -* @g1 (R_src a) (R_tgt a) (Q a) (ps a) (pt a) (itr_src a) (itr_tgt a) (ths a) (im_src a) (im_tgt a) (st_src a) (st_tgt a))) ** P a) (isim r g0 (Q a) (ps a) (pt a) (itr_src a) (itr_tgt a) (ths a) (im_src a) (im_tgt a) (st_src a) (st_tgt a)))
+                                                    (∀ a, P a -* @g1 (R_src a) (R_tgt a) (Q a) (itr_src a) (itr_tgt a) (ths a) (im_src a) (im_tgt a) (st_src a) (st_tgt a))) ** P a) (isim r g0 (Q a) (itr_src a) (itr_tgt a) (ths a) (im_src a) (im_tgt a) (st_src a) (st_tgt a)))
     :
-    (forall a, bi_entails (P a) (isim r g0 (Q a) (ps a) (pt a) (itr_src a) (itr_tgt a) (ths a) (im_src a) (im_tgt a) (st_src a) (st_tgt a))).
+    (forall a, bi_entails (P a) (isim r g0 (Q a) (itr_src a) (itr_tgt a) (ths a) (im_src a) (im_tgt a) (st_src a) (st_tgt a))).
   Proof.
     i. rr. autorewrite with iprop. ii. clear WF.
     revert a r0 H r_ctx WF0. gcofix CIH. i.
     epose (fun R_src R_tgt (Q: R_src -> R_tgt -> shared_rel)
-               ps pt itr_src itr_tgt ths im_src im_tgt st_src st_tgt =>
+               itr_src itr_tgt ths im_src im_tgt st_src st_tgt =>
              @iProp_intro _ (fun r_own => forall r_ctx (WF: URA.wf (r_own ⋅ r_ctx)),
-                                 gpaco9 gf (cpn9 gf) r0 r0 R_src R_tgt (liftRR Q) ps pt r_ctx itr_src itr_tgt (ths, im_src, im_tgt, st_src, st_tgt)) _).
+                                 gpaco9 gf (cpn9 gf) r0 r0 R_src R_tgt (liftRR Q) false false r_ctx itr_src itr_tgt (ths, im_src, im_tgt, st_src, st_tgt)) _).
     hexploit (COIND i a). subst i. clear COIND. i.
     rr in H. autorewrite with iprop in H. hexploit H.
     { instantiate (1:=r1). eapply URA.wf_mon; eauto. }
